raft/simulator/raft/RaftSimul.ml
@@ -5,8 +5,16 @@ open Core
 open Simulator
 open RaftReplicaEx
 
+let char_list2string l = Batteries.String.of_list l
+
+let print_state state = char_list2string (state2string (sm_state state))
+
 let to_replica n = { id = Obj.magic (Raftreplica (Obj.magic n));
-                     replica = local_replica (Obj.magic n) }
+                     replica = local_replica false (Obj.magic n) }
+
+let to_leader n = { id = Obj.magic (Raftreplica (Obj.magic n));
+                     replica = local_replica true (Obj.magic n) }
+
 
 let destination2string (n : name) : string =
   match Obj.magic n with
@@ -17,22 +25,22 @@ class ['a, 'b, 'c, 'd] raft c = object(self)
   inherit ['a, 'b, 'c, 'd] simulator c
 
   method create_replicas =
-    replicas#set_replicas [to_replica 0; to_replica 1; to_replica 2; to_replica 3];
+    replicas#set_replicas [to_leader 0; to_replica 1; to_replica 2; to_replica 3];
 
   method mk_request (timestamp : int) (request : int) =
-    let cmd = 0 in
+    let cmd = 12 in
     let term = 0 in
     let client = Obj.magic conf.client_id in
-    RequestMsg (Req(client, cmd, term))
+    RequestMsg (Req(client, (Obj.magic cmd), term))
 
   method run_replicas (inflight : directedMsgs) : directedMsgs =
     match inflight with
     | [] -> []
     | dm :: dms ->
-      print_info (kCYN) "Procesing" (Batteries.String.of_list (directedMsg2string dm));
       match dm.dmDst with
       | [] -> self#run_replicas dms
       | id :: ids ->
+        print_info (kCYN) "Procesing" (char_list2string (directedMsg2string dm));
         let dm' = { dmMsg = dm.dmMsg; dmDst = ids; dmDelay = dm.dmDelay } in
         match replicas#find_replica id with
         | None ->
@@ -40,25 +48,26 @@ class ['a, 'b, 'c, 'd] raft c = object(self)
           let failed_to_deliver = { dmMsg = dm.dmMsg; dmDst = [id]; dmDelay = dm.dmDelay } in
           failed_to_deliver :: self#run_replicas (dm' :: dms)
         | Some rep ->
-          print_info (kGRN) "Input message"
-            (Batteries.String.of_list(msg2string (Obj.magic dm.dmMsg)));
+          print_info (kGRN) (destination2string id ^ " | Input message")
+            (char_list2string (msg2string (Obj.magic dm.dmMsg)));
+          print_endline (char_list2string (state2string rep.replica.sm_state));
           let (rep',dmsgs) = lrun_sm rep.replica (Obj.magic dm.dmMsg) in
           print_info (kCYN) "Done" "";
           replicas#replace_replica id rep';
+          print_endline (char_list2string (state2string rep'.sm_state));
           self#run_replicas (dm' :: dms @ dmsgs)
 
   method run_client timestamp max avg printing_period =
     let req = self#mk_request (Obj.magic timestamp) 17 in
     let inflight = [{ dmMsg = Obj.magic req; dmDst = [c.primary]; dmDelay = 0 }] in
     let t = Prelude.Time.get_time () in
-    print_endline (Batteries.String.of_list (directedMsgs2string inflight));
+    print_info (kBLU) "Start" (char_list2string (directedMsgs2string inflight));
     let failed_to_deliver = self#run_replicas inflight in
     let d = Prelude.Time.sub_time (Prelude.Time.get_time ()) t in
     let new_avg = Prelude.Time.div_time (Prelude.Time.add_time (Prelude.Time.mul_time avg  (timestamp - 1)) d) timestamp in
-    let s = Batteries.String.of_list (directedMsgs2string failed_to_deliver) in
-    (match s with
-     | "" -> ()
-     | s' -> print_err s' ~case:"Failed to deliver: " ());
+    (match failed_to_deliver with
+     | [] -> ()
+     | s' -> print_err (char_list2string (directedMsgs2string s')) ~case:"Failed to deliver: " ());
     (if timestamp mod printing_period = 0 then
        print_res timestamp d new_avg
      else ());
@@ -73,6 +82,6 @@ let _ =
     protocol = "Raft";
     client_id = 0;
     private_key = lookup_client_sending_key (Obj.magic 0);
-    primary = Obj.magic (Raftreplica (Obj.magic 0)) (* type: name *)
+    primary = Obj.magic (Raftreplica (Obj.magic 1)) (* type: name *)
   } in
   c#run
