raft/protocols/Raft/RaftHeader.v
@@ -7,6 +7,7 @@
 Require Export Velisarios.Quorum.
 (* the process module provides the abstraction which is implemented by the protocols *)
 Require Export Velisarios.Process.
+Require Export String.
 
 (*! abstract topology !*)
 (** This section defines the topology of raft which is modeled as an agent
@@ -56,6 +57,10 @@ Section RaftHeader.
         (* this should be the base timerout for the leader election
          * where no followers should start at the same moment with voting. *)
         base_timeout : nat;
+        (* the content type for the log *)
+        content_type : Set;
+        (* get a textual representation from the content *)
+        content2string : content_type -> string;
       }.
 
   (** Declares the context type class as new variable with implicit
@@ -82,26 +87,19 @@ Section RaftHeader.
    * as natural number *)
   | Raftclient (n : Client).
 
-  (** A maybe to simple implmentation to unwrap some raft node by using the sum type. **)
-  Definition n2r (n : Raftnode) : Rep + Client :=
+  (* extract the replica of some node *)
+  Definition node2rep (n : Raftnode) : option Rep :=
     match n with
-    | Raftreplica n => inl n
-    | Raftclient n => inr n
+    | Raftreplica n => Some n
+    | _ => None
     end.
 
-  (* extract the replica of some node *)
-  (* Definition node2rep (n : Raftnode) : option Rep := *)
-  (*   match n with *)
-  (*   | Raftreplica n => Some n *)
-  (*   | _ => None *)
-  (*   end. *)
-
-  (* (* extract the client of some node *) *)
-  (* Definition client2rep (n : Raftnode) : option Client := *)
-  (*   match n with *)
-  (*   | Raftclient n => Some n *)
-  (*   | _ => None *)
-  (*   end. *)
+  (* extract the client of some node *)
+  Definition client2rep (n : Raftnode) : option Client :=
+    match n with
+    | Raftclient n => Some n
+    | _ => None
+    end.
 
   (** Prove that raft nodes have decidable equality like the one from Leibnitz. **)
   Lemma RaftnodeDeq : Deq Raftnode.
@@ -119,7 +117,100 @@ Section RaftHeader.
   (** Bind the real node definition as instance to the abstract definition from veliarios. **)
   Global Instance Raft_I_Node : Node := MkNode Raftnode RaftnodeDeq.
 
-  (*! Here are the definitions for the types used in within the messages !*)
+  (*! TODO: Add more notes to this section!*)
+  (*! Quorum instance !*)
+  Lemma Raftreplica_inj : injective Raftreplica.
+  Proof.
+    introv h; ginv; auto.
+  Qed.
+
+  Global Instance Raft_I_Quorum : Quorum_context :=
+    MkQuorumContext
+      Rep
+      num_replicas
+      rep_deq
+      reps2nat
+      reps_bij
+      Raftreplica
+      Raftreplica_inj.
+
+  (* can we have something like this? *)
+  Definition rep2node := Rep -> node_type.
+
+  (*! TODO: Add more notes to this section !*)
+  (*! More about nodes !*)
+  (* 0 is less than 2*F+1 *)
+  Definition nat_n_2Fp1_0 : nat_n num_replicas.
+  Proof.
+    exists 0.
+    apply leb_correct.
+    unfold num_replicas.
+    omega.
+  Defined.
+
+  Definition replica0 : Rep := bij_inv reps_bij nat_n_2Fp1_0.
+
+  (*Eval simpl in (name_dec (PBFTreplica replica0) (PBFTreplica replica0)).*)
+
+  (* We'll return the node as given by our bijection if n < num_nodes,
+     otherwise we return a default value (replica0)
+   *)
+  Definition nat2rep (n : nat) : Rep.
+  Proof.
+    destruct reps_bij as [f a b].
+    destruct (lt_dec n num_replicas) as [d|d].
+    - exact (f (mk_nat_n d)). (* here we now that n < num_replicas so we can use our bijection *)
+    - exact replica0. (* here num_replicas <= n, so we return a default value: replica0 *)
+  Defined.
+
+
+  Definition reps : list Rep := (* nodes. *)
+   mapin
+      (seq 0 num_replicas)
+      (fun n i => bij_inv reps_bij (mk_nat_n (seq_0_lt i))).
+
+  Definition nreps : list name := map Raftreplica reps.
+
+  Lemma reps_prop : forall (x : Rep), In x reps.
+  Proof.
+    exact nodes_prop.
+  Qed.
+
+  Definition clients : list Client :=
+    mapin
+      (seq 0 num_clients)
+      (fun n i => bij_inv clients_bij (mk_nat_n (seq_0_lt i))).
+
+  Definition nclients : list name := map Raftclient clients.
+
+  Lemma clients_prop : forall (x : Client), In x clients.
+  Proof.
+    introv.
+    unfold clients.
+    apply in_mapin.
+
+
+    remember (clients2nat x) as nx.
+    destruct nx as [nx condnx].
+
+    pose proof (leb_complete _ _ condnx) as c.
+
+    assert (In nx (seq O num_clients)) as i.
+    { apply in_seq; omega. }
+
+    exists nx i; simpl.
+
+    unfold mk_nat_n.
+    unfold bij_inv.
+    destruct clients_bij.
+    pose proof (bij_id1 x) as h.
+    rewrite <- Heqnx in h; subst; simpl.
+
+    f_equal; f_equal.
+    apply UIP_dec; apply bool_dec.
+  Qed.
+
+  (*! Here are the definitions for the types used in within the messages and states !*)
 
   (*! Terms and progress !*)
   (** Within this protocol the global time is divided into chunks called terms.
@@ -150,7 +241,7 @@ Section RaftHeader.
     destruct (deq_nat n n0); prove_dec.
   Defined.
 
-  (** The first term start with zero. **)
+  (** On boot the first term start with zero. **)
   Definition initial_term := term 0.
 
   (** Test wether term 1 is lesser or equal than term 2. **)
@@ -165,13 +256,146 @@ Section RaftHeader.
   Definition max_term (t1 t2 : Term) : Term :=
     if TermLe t1 t2 then t2 else t1.
 
+  (*! next index !*)
+  (** The next index is a list of the tuple server id and the
+   ** next possible index for the server.
+   ** The leaders initializes this list every time to last log index + 1.
+   ** The index of a node is increased monotonically if an append entries
+   ** message is send to the node **)
+  Inductive NextIndex :=
+  | next (rep : Rep) (next_index : nat).
+
+  (** A convient notation for a list of next indices **)
+  Notation nindex := (list NextIndex).
+
+
+  (** Create a new next index list out of list of nodes and an initial value **)
+  Fixpoint create_next_index (reps : list Rep) (n : nat) : nindex :=
+    match reps with
+    | [] => []
+    | r :: rs => next r n  :: create_next_index rs n
+    end.
+
+  (** Increase some index **)
+  Definition increase_next_index_e (n : NextIndex) : NextIndex :=
+    match n with
+    | next r ni => next r (ni + 1)
+    end.
+
+  (** Increase an element in the next index list **)
+  Fixpoint increase_next_index (l : nindex) (rep : Rep) : nindex :=
+    match l with
+    | [] => l (* return list if last element reached *)
+    | (next r _) as x :: xs => if (rep_deq r rep)
+                          then increase_next_index_e x :: xs
+                          else x :: increase_next_index xs rep
+    end.
+
+  (** Return some index if the node is found **)
+  Fixpoint get_next_index (l : nindex) (rep : Rep) : option nat :=
+    match l with
+    | [] => None (* the node is not found *)
+    | (next r i) :: xs => if (rep_deq r rep)
+                        then Some i
+                        else get_next_index xs rep
+    end.
+
+  (*! match index !*)
+  (** The list of match indices is basically the same as the list of next indices
+   ** so the definition are just wrappers about the next index functions.
+   ** The next index stores for a server the index which it knows is replicated by the
+   ** node. One can see this list as mechanism to track the which server has applied
+   ** an append entries message to its local log. **)
+  Notation mindex := (list NextIndex).
+
+  Definition create_match_index (reps : list Rep) : mindex := create_next_index reps 0.
+
+  Definition increase_match_index (l : mindex) (rep : Rep) := increase_next_index l rep.
+
+  Definition get_match_index (l : mindex) (rep : Rep) := get_next_index l rep.
+
+  (*! Log !*)
+  (** An entry in the log takes the term where it is added to the log and
+   ** the content which gets added to the log.
+   ** TODO: The content is a parametrized type.
+   **
+   ** Log matching property
+   ** 1. If 2 entries in different logs have the same index and term they store the same command.
+   ** 2. If 2 entries in different logs have same index and term, then the preceding
+   **    entries are identical in the logs
+   ** To keep the semantics clear, "log," denotes the node internal list of entries and "list Entry"
+   ** denotes the new requested entries messaged through append entries calls. **)
+
+  (** An entry is a typeclass which gets parametrized over its content. **)
+  Record Entry :=
+    MkEntry
+      {
+        entry_term : Term;
+        entry : content_type;
+      }.
+
+  (** Create a new content entry from the type, entry term and content **)
+  Definition new_entry (t : Term) (c : content_type) :=
+    MkEntry
+      t
+      c.
+
+  (** Define an abbreviation for the entry list. The comma is enforced by coq. **)
+  Notation "log," := (list Entry) (at level 100).
+
+  (** Search for the last entry and return its entry term. **)
+  Fixpoint get_last_log_term (l : log,) : Term :=
+    match l with
+    | [] => term 0
+    | {|entry_term := t|}  :: [] => t
+    | _ :: xs => get_last_log_term xs
+    end.
+
+  (** Utility function which counts the elements in a log. **)
+  Fixpoint get_last_log_index_util (l : log,) (n : nat) :=
+    match l with
+    | [] => n
+    | _ :: xs => get_last_log_index_util xs (n+1)
+    end.
+
+  (** The first index is 1 **)
+  Definition get_last_log_index (l : log,) : nat := get_last_log_index_util l 1.
+
+  (** Check if at position i the entry has the entry term "t". **)
+  Fixpoint check_last_log (i : nat) (t : Term) (l : log,) : bool :=
+    match l with
+    | [] => true (* if the log is empty any new entry is accepted *)
+    | {|entry_term := t'|} :: [] => if (TermDeq t t') then true else false
+    | _ :: xs => check_last_log (i - 1) t xs
+    end.
+
+  (** Take e elements from the log. Start from the end of the list. **)
+  Fixpoint take_from_log_util (e : nat) (l : log,) :=
+    match l with
+    | [] => ([], 0)
+    | x :: xs =>
+      let (l, i) := take_from_log_util e xs in
+      if (i <? e) then (x :: l, i+1) else (l,i)
+    end.
+
+  Definition take_from_log (e : nat) (l : log,) :=
+    let (l, i) := take_from_log_util e l in l.
+
+  (** Append new entries to a log  **)
+  Fixpoint append2log (l : log,) (e : list Entry) :=
+    match e with
+    | [] => l
+    | x :: xs => x :: append2log l xs
+    end.
+
+
   (*! Request !*)
   (** A request is issued by some client and contains the client itself for the response message
    *+ and the command issued to replicate as well as the term number to participate. **)
   Inductive Request :=
-  | Req (client : Client) (command : nat) (term : Term).
+  | Req (client : Client) (command : content_type) (term : Term).
 
-
+  (*! Heartbeat and Log replication !*)
   (** The append entries type has two function within the protocol. First it serves as a
    ** heartbeat to prevent follower to suspect the leader is faulty and second it is used to
    ** issue a log replication by some follower.
@@ -181,17 +405,19 @@ Section RaftHeader.
   Inductive AppendEntries :=
   | Heartbeat
   | Replicate (term : Term) (leader : Rep) (last_log_index : nat)
-              (last_log_term : Term) (commit_index : nat) (entry : list nat).
+              (last_log_term : Term) (commit_index : nat) (entry : list Entry).
 
+  (*! Election !*)
   (** A vote is issued during the leader election. The candidate provides
    ** itself, the current term and the index of the last stored log and
    ** it's term number. **)
   Inductive RequestVote :=
   | Vote (term : Term) (candidate : Rep) (last_log_index : nat) (last_log_term : Term).
 
-    (** The result type provides the different results used within the protocol. **)
-    Inductive Result :=
-    (** The leader sends the client the response if his state machine. **)
+  (*! Results !*)
+  (** The result type provides the different results used within the protocol. **)
+  Inductive Result :=
+  (** The leader sends the client the response if his state machine. **)
   | ClientRes (result : nat)
   (** The follower responses to the leader if the issued requests succeds and
    ** the current term to update the leader. **)
@@ -231,7 +457,10 @@ Section RaftHeader.
   (* The response vote messages is returned by processing some request vote message.
    * It indicates to the requesting client wether it recieves a vote from this
    * node or not. *)
-  | ResponseVoteMsg (result : Result).
+  | ResponseVoteMsg (result : Result)
+  (* The forwarding is used if some client send a request to a none leader replica.
+   * It encapsulates the message and sends it to the current leader. *)
+  | ForwardMsg (msg : Raftmsg).
 
   (** Bind the implemented messages to the abstract velisarios type class. **)
   Global Instance Raft_I_Msg : Msg := MkMsg Raftmsg.
@@ -247,9 +476,11 @@ Section RaftHeader.
     | AppendEntriesResultMsg _ => MSG_STATUS_PROTOCOL
     | RequestVoteMsg _         => MSG_STATUS_PROTOCOL
     | ResponseVoteMsg _        => MSG_STATUS_PROTOCOL
+    | ForwardMsg _             => MSG_STATUS_PROTOCOL
     end.
 
   (** Bind the real message states to the abstract definition. **)
   Global Instance Raft_I_get_msg_status : MsgStatus := MkMsgStatus Raftmsg2status.
 
 End RaftHeader.
+
