raft/protocols/Raft/Raft.v
@@ -21,9 +21,16 @@ Section Raft.
   (** Redeclare the general system context as new local variable. **)
   Context { raft_context : RaftContext }.
 
+  (** redeclare the notations **)
+  Notation Nindex := (list NextIndex).
+  Notation Mindex := (list NextIndex).
+  Notation Log := (list Entry).
+  Notation Commit_log := (list Entry).
+
   (*! Leader state !*)
   (** The leader state indicates the node as leader and is reinitialized after every
    ** election round. **)
+
   Record RaftLeaderState :=
     Build_Leader_State
       {
@@ -32,44 +39,52 @@ Section Raft.
         (* Volatile; reset after election -
          * The list of followers and the next possible index to send to the follower.
          * Try list index as node marker -> (node_num, next_index)*)
-        next_index : list nat;
+        next_index : Nindex;
         (* Volatile; reset after election -
          * The list of servers and their index of the highest log entry.
          * Try the list index as a marker for the node id. *)
-        match_index : list nat;
+        match_index : Mindex;
       }.
 
   (** This definition is used to initialize the network, because
    ** their is no leader in the beginning. **)
-  Definition initial_leader_state : RaftLeaderState :=
+  Definition no_leader_state : RaftLeaderState :=
     Build_Leader_State false [] [].
 
-  (** Build a list with some default number. **)
-  Fixpoint build_follower_list (arg : nat) (followers : nat) : list nat :=
-    match followers with
-    | O => []
-    | S n => [arg] ++ build_follower_list arg n
-    end.
+  (** This definition is used only for testing. It creates an initial leader *)
+  (*  ** with a provided follower network. **)
+  Definition init_leader_state (followers : list nat) : RaftLeaderState :=
+    let reps := List.map nat2rep followers in
+    Build_Leader_State true
+                       (create_next_index reps 0)
+                       (create_match_index reps).
 
   (** This definition reinitializes the node that has won the leader election. **)
-  Definition after_election_leader (next_index : nat) (followers : nat) : RaftLeaderState :=
+  Definition after_election_leader (next_index : nat) (followers : list Rep) : RaftLeaderState :=
     Build_Leader_State true
-                       (build_follower_list next_index followers)
-                       (build_follower_list 0 followers).
+                       (create_next_index followers next_index)
+                       (create_match_index followers).
 
   (*! Node State !*)
   (** The state describes the parts that are persistent on all nodes. **)
   Record RaftState :=
     Build_State
       {
-        (* The last term the node has seen. *)
+        (* The last term the node has seen, this should be persitent over crashes. *)
         current_term : Term;
         (* The candidate this node voted for the current term or null if none *)
         voted_for : (option nat);
-        (* The replicated log data. !Use nat at the beginning! *)
-        log : list nat;
-        (* Volatile - The last log index known to be committed. *)
+        (* The replicated log data which should be persitent over crashes
+         * !Use nat at the beginning! *)
+        log : Log;
+        (* Volatile - The last log index known to be committed.
+         * The index provides information to which request the global state machine
+         * has applied the requests. *)
         commit_index : nat;
+        (* Since we don't implement a real state machine where the commited logs
+         * gets applied (out of scope) a second list is used as dummy to show the mechanics.
+         * If a majority agrees on a log entry the entry gets copied to the commited_log. *)
+        committed : Commit_log;
         (* Volatile - The last log index applied to the state machine. *)
         last_applied : nat;
         (* the timeout in secs after which a new election is triggered.
@@ -80,19 +95,57 @@ Section Raft.
         sm_state : RaftSM_state;
         (* The leader state if the node is the leader *)
         leader : RaftLeaderState;
+        (* The term leader *)
+        current_leader : (option Rep);
+        (* the list of other servers excluding this one *)
+        nodes : list nat;
       }.
 
   (** The initial state for all nodes. **)
-  Definition initial_state (r : Rep) : RaftState :=
+  Definition initial_state : RaftState :=
     Build_State
       initial_term (* zero at first boot *)
       None (* voted for no one. *)
       [] (* no log entries stored *)
       0 (* no commit done *)
+      [] (* empty commited log *)
       0 (* nothing applied to state machine *)
       5 (* some way of defining an offset is needed *)
       RaftSM_initial_state (* defined within the raft context *)
-      initial_leader_state.
+      no_leader_state (* at default no one is leader *)
+      None (* set leader to none *)
+      [].
+
+  (** An initial state for replicas with the leader set to replica 0. **)
+  Definition initial_faked_leader_state : RaftState :=
+    Build_State
+      initial_term (* zero at first boot *)
+      None (* voted for no one. *)
+      [] (* no log entries stored *)
+      0 (* no commit done *)
+      [] (* empty commited log *)
+      0 (* nothing applied to state machine *)
+      5 (* some way of defining an offset is needed *)
+      RaftSM_initial_state (* defined within the raft context *)
+      no_leader_state (* at default no one is leader *)
+      (Some (nat2rep 0)) (* set leader to 0 *)
+      [] (* empty list of nodes *).
+
+
+  (** An initial leader state which should only used for testing. **)
+  Definition initial_leader_state : RaftState :=
+    Build_State
+      initial_term (* zero at first boot *)
+      None (* voted for no one. *)
+      [] (* no log entries stored *)
+      0 (* no commit done *)
+      [] (* empty commited log *)
+      0 (* nothing applied to state machine *)
+      5 (* some way of defining an offset is needed *)
+      RaftSM_initial_state (* defined within the raft context *)
+      (init_leader_state [1, 2, 3]) (* define as leader with 3 followers *)
+      (Some (nat2rep 0)) (* set leader to 0 for testing *)
+      [1, 2, 3] (* empty list of nodes *).
 
   (*! State transitions !*)
   (** If some leader is byzantine a new election starts and the term number is increased **)
@@ -102,11 +155,66 @@ Section Raft.
       (voted_for s)
       (log s)
       (commit_index s)
+      (committed s)
       (last_applied s)
       (node_timeout s)
       (sm_state s)
-      (leader s).
+      (leader s)
+      (current_leader s)
+      (nodes s).
 
+  (** replace the nodes log **)
+  Definition update_log (s : RaftState) (l : list Entry) : RaftState :=
+    Build_State
+      (current_term s)
+      (voted_for s)
+      l
+      (commit_index s)
+      (committed s)
+      (last_applied s)
+      (node_timeout s)
+      (sm_state s)
+      (leader s)
+      (current_leader s)
+      (nodes s).
+
+    (** replace the commit index **)
+  Definition update_commit_log (s : RaftState) (ci : nat) (l : Commit_log) : RaftState :=
+    Build_State
+      (current_term s)
+      (voted_for s)
+      (log s)
+      ci
+      l
+      (last_applied s)
+      (node_timeout s)
+      (sm_state s)
+      (leader s)
+      (current_leader s)
+      (nodes s).
+
+  Definition update_leader (s : RaftState) (l : Rep) : RaftState :=
+    Build_State
+      (current_term s)
+      (voted_for s)
+      (log s)
+      (commit_index s)
+      (committed s)
+      (last_applied s)
+      (node_timeout s)
+      (sm_state s)
+      (leader s)
+      (Some l)
+      (nodes s).
+
+
+  (*! Utilities !*)
+
+  (** TODO: This seems like vodoo, at the moment, where does reps come from. **)
+  Definition other_replicas (r : Rep) : list Rep := remove_elt rep_deq r reps.
+  Definition other_names (r : Rep) : list name := map Raftreplica (other_replicas r).
+
+  Definition leading (s : RaftState) : bool := (is_leader (leader s)).
 
   (*! The message handling - Update function !*)
   (** Each possible transition has it's own handle function for the input message.
@@ -114,29 +222,176 @@ Section Raft.
    ** actual implementation provide higher types if you need multiple arguments
    ** to handle the message. **)
 
-  (** L - Handle client input to the system. **)
-  Definition Rafthandle_request (slf : Rep) : Update RaftState Request DirectedMsgs :=
-    fun state _ => (Some state, []).
+  (*! Internal Forwarding !*)
+  (** The internal forwarding mechanism is a fairly simple one.
+   ** 1. If a client request is send to the wrong node it gets forwarded to the node
+   ** this node assumes to be the leader.
+   ** 2. If this node has no leader (newly started network) it currently drops the request.
+   ** 3. The reciever forwards the message if it is not the leader
+   ** 4. Otherwise, it unpacks all messages and sends the innerst message to itself **)
+  Definition create_forward_msg (s : option Rep) (o : Raftmsg) : DirectedMsgs :=
+    match s with
+      (* we have no new current leader, maybe the system was recently initialized and
+       * no leader is elected yet. TODO: Ignore the message at the moment *)
+    | None => []
+    | Some l => [MkDMsg (ForwardMsg o) [Raftreplica l] 0]
+    end.
 
-    (** Cl - Handle client response - currently nothing **)
-  Definition Rafthandle_response (slf : Rep) : Update RaftState Result DirectedMsgs :=
-    fun state _ => (Some state, []).
+  (** Unwrap all possible wrapped forwarded messages and return the original message. **)
+  Fixpoint unpack_forwards (f : Raftmsg) : Raftmsg :=
+    match f with
+    | ForwardMsg f => unpack_forwards f
+    | f => f
+    end.
+
+  (** L - Handle fowarded message - unpack and send original message to self. **)
+  Definition Rafthandle_forward_msg (slf : Rep) : Update RaftState Raftmsg DirectedMsgs :=
+    fun state f =>
+      if leading state then
+        (* maybe there is a better way of handling this. *)
+        let msg := unpack_forwards f in
+        (Some state, [MkDMsg msg [(Raftreplica slf)] 0])
+      (* Either forward the message to the current leader or ignore it.
+       * Maybe a TODO to handle the first encountered messages if there is no leader. *)
+      else (Some state, (create_forward_msg (current_leader state) f)).
+
+  (*! Log replication !*)
+  (** 1. If a node gets a request and it is not the leader it forwards the request.
+   ** 2. If the node is the leader
+   ** 2.1 It stores the request in its internal log
+   ** 2.2 It sends append entries messages to all its followers
+   ** 3. A follower applies the entries to it's internal log if the index is free or a wrong entry is present.
+   ** 3.1 It ignores the entries if the index is present and the terms are matching
+   ** 4. The follower updates the commit_index and commits log entries to the commited_log
+   ** 5. The follower repsonds to the leader with it's result and the current term
+   ** 6. If the leader gets a majority of successfull repsonses from the followers
+   **    it commits the log entry to the commited_log. **)
+
+  (** Create the replication messages which are send to the followers
+   ** To make this easy the request sends a nat as cmd to the leader and
+   ** the leader converts this into a single entry list for the log replication. **)
+  Definition create_append_msg (slf : Rep) (s : RaftState) (entries: list Entry) : DirectedMsgs :=
+    let leader := leader s in
+    let llt := get_last_log_term (log s) in
+    let lli := get_last_log_index (log s) in
+    let msg := Replicate (current_term s) slf lli llt (commit_index s) entries in
+    [MkDMsg (AppendEntriesMsg msg) (other_names slf) 0].
+
+  (** 1. If the next used log index is equal to the internal log index
+   ** 1.1 check if the terms of the entries are matching and
+   ** 1.1.1 if the terms are equal do nothing
+   ** 1.1.2 if the terms are unequal take only the log until the last_log_index and append the new entries
+   ** 2. If the next used log index is free append the entries **)
+  Definition append_entries2log (entries : list Entry) (lli : nat) (t : Term) (s : RaftState) :=
+    let log := log s in
+    let last_index := get_last_log_index log in
+    if ((lli + 1) ==  last_index) then
+      (* an entry exists, now check if terms are matching *)
+      let last_term := get_last_log_term log in
+      if (TermDeq t last_term) then
+        (* the terms are matching, we assume the entry is correct *)
+        []
+      else (* delete the requested index and all entries which follow this one *)
+        let log' := take_from_log (lli + 1) log in
+        append2log log' entries
+    else append2log log entries.
+
+  (** If the internal commit index is lower than the provided one
+   ** return min (provided_commit_index, last_log_index) **)
+  Definition new_commit_index (s : RaftState) (ci : nat) :=
+    if ((commit_index s) <? ci) then
+      let lli := get_last_log_index (log s) in
+      min ci lli
+    else (commit_index s). (* if the nodes index is higher the paper doesn't handle this case *)
+
+  (** Check if there are new commits and apply them to the local committed log. **)
+  Definition commit (s : RaftState) (ci : nat) :=
+    let new_ci := new_commit_index s ci in
+    let log := take_from_log new_ci (log s) in
+    (update_commit_log s new_ci log).
+
+  (** L - Handle client input to the system. **)
+  (** Forward the message if the request reaches the wrong node.
+   ** As leader generate the entries from the request and apply the entries to the
+   ** internal log. Afterwards send AppendEntries messages to the followers. **)
+  Definition Rafthandle_request (slf : Rep) : Update RaftState Request DirectedMsgs :=
+    fun state r =>
+      if leading state then
+        (* We are the leader *)
+        match r with
+        | Req client cmd t =>
+          let entry := [new_entry (term (current_term state)) cmd] in
+          (* create the replication messages for all leaders *)
+          let dmsgs := create_append_msg slf state entry in
+          (* apply the messages to your own log
+           * Paper missing description about how to add as a leader, currently use the same fn as the followers *)
+          let lli := get_last_log_index (log state) in
+          let new_state := (update_log state (append_entries2log entry lli (current_term state) state)) in
+          (Some new_state, dmsgs)
+        end
+      else
+      (* Some node that forwards *)
+        let msg := create_forward_msg (current_leader state) (RequestMsg r) in
+        (Some state, msg).
 
   (** F - Handle append entries messages which are used as heartbeat and log replication. **)
+  (** As a leader ignore the message.
+   ** As a follower
+   ** 1. Check if the message is a heartbeat or replication
+   ** 2. Ignore heartbeats at the moment
+   ** 3. Check if the entries could be applied to the internal log
+   ** 3.1 Ignore the request if the current term doesn't match or the entry is already there (index + term)
+   ** 3.2 Apply the entries to the internal log by removing false entries and response with success and the current term **)
   Definition Rafthandle_append_entries (slf : Rep) : Update RaftState AppendEntries DirectedMsgs :=
-    fun state _ => (Some state, []).
+    fun state msg =>
+      if leading state then (Some state, []) (* this shouldn't happen *)
+      else
+        match msg with
+        (* leader timeout reset *)
+        | Heartbeat => (Some state, []) (* TODO: ignore election at the moment *)
+        (* log replication *)
+        | Replicate t l lli llt ci entries =>
+          if (TermLt t (current_term state)) then
+            (* reply false if the replication term is lower than the current term *)
+            let result := AppendEntriesRes false (current_term state) in
+            (Some state, [MkDMsg (AppendEntriesResultMsg result) [Raftreplica l] 10])
+          else
+            if (negb (check_last_log lli llt (log state))) then
+              (* reply false if the last log index or term does not match *)
+              let result := AppendEntriesRes false (current_term state) in
+              (Some state, [MkDMsg (AppendEntriesResultMsg result) [Raftreplica l] 20])
+            else
+              (* handle the replication request *)
+              let new_log := append_entries2log entries lli t state in
+              let result := AppendEntriesRes true (current_term state) in
+              let s := (update_log state new_log) in
+              let s' := (commit s ci) in
+              let s'' := (update_leader s' l) in
+              (Some s'', [MkDMsg (AppendEntriesResultMsg result) [Raftreplica l] 0])
+        end.
 
   (** L - Handle results messages from followers. **)
   Definition Rafthandle_append_entries_result (slf : Rep) : Update RaftState Result DirectedMsgs :=
-    fun state _ => (Some state, []).
+    fun state r =>
+      if leading state then
+        (* let c := [Raftclient client] in *)
+        (* (Some state, [MkDMsg (ResponseMsg (ClientRes cmd)) c 0]) *)
+        (Some state, [])
+    
+      else (Some state, []). (* this shoudln't happen *)
 
-    (** C - Handle incoming votes from candidates. **)
+  (** C - Handle incoming votes from candidates. **)
   Definition Rafthandle_request_vote (slf : Rep) : Update RaftState RequestVote DirectedMsgs :=
     fun state _ => (Some state, []).
 
-    (** C - Handle incoming voting results from candidates. **)
+  (** C - Handle incoming voting results from candidates. **)
   Definition Rafthandle_response_vote (slf : Rep) : Update RaftState Result DirectedMsgs :=
     fun state _ => (Some state, []).
+
+  (** Cl - The client handles the response from a node - currently nothing **)
+  Definition Rafthandle_response (slf : Rep) : Update RaftState Result DirectedMsgs :=
+    fun state _ => (Some state, []).
+
 
   (** The main update function which calls the appropriate handler function
    ** for the incoming message type. **)
@@ -149,6 +404,7 @@ Section Raft.
       | AppendEntriesResultMsg d => Rafthandle_append_entries_result slf state d
       | RequestVoteMsg d => Rafthandle_request_vote slf state d
       | ResponseVoteMsg d => Rafthandle_response_vote slf state d
+      | ForwardMsg msg => Rafthandle_forward_msg slf state msg
       end.
 
   (*! System definitions !*)
@@ -156,7 +412,13 @@ Section Raft.
   Definition RaftreplicaSM (slf : Rep) : MStateMachine _ (* let the compiler guess ? *) :=
     mkSM
       (Raftreplica_update slf)
-      (initial_state slf).
+      (initial_faked_leader_state).
+
+  (** This binding should only used for testing. **)
+  Definition RaftLeaderreplicaSM (slf : Rep) : MStateMachine _ (* let the compiler guess ? *) :=
+    mkSM
+      (Raftreplica_update slf)
+      (initial_leader_state).
 
   (* match node names with state machines *)
   Definition Raftnstate (n : name) :=
