raft/protocols/Raft/RaftHelper.v
@@ -1,0 +1,34 @@
+(*!
+ * This file defines general helper functions which are used
+ * throughout the code.
+ !*)
+
+Section RaftHelper.
+
+  (** concat a list of string to one string. **)
+  Fixpoint str_concat (l : list String.string) : String.string :=
+    match l with
+    | [] => ""
+    | s :: ss => String.append s (str_concat ss)
+    end.
+
+  (** auxilary function which converts a list of some type to its representation. **)
+  Fixpoint list2string_aux {A : Type} (l : list A) (s : A -> string) : string :=
+    match l with
+    | [] => ""
+    | [x] => s x
+    | x :: xs => str_concat [s x, ", ", list2string_aux xs s]
+    end.
+
+  (** Convert a list to a string according the rules. **)
+  Definition list2string {A : Type} (l : list A) (s : A -> string) : string :=
+    str_concat ["[", list2string_aux l s, "]"].
+
+  (** The next three functions are placeholder functions which are later
+   ** replaced by real ocaml function within the extraction process. **)
+  (** line feed **)
+  Definition LF : string := String (ascii_of_nat 10) "".
+  Definition print_endline : string -> unit := fun _ => tt.
+  Definition nat2string (n : nat) : string := "-".
+
+End RaftHelper.
